---
title: "Exercise 2.1"
subtitle: "Consumption Innovations"
---
<a class="return-button" href="index.qmd">â¬… Return</a>

## Problem

In the economy with AR(1) endowment shocks studied in section 2.2, we found that $E_{t}c_{t+1}=c_{t}$, which means that $c_{t+1} = c_{t}+\mu_{t+1}$, where $\mu_{t+1}$ is a white noise process that is unforecastable given information available in t. Derive the innovation $\mu_{t+1}$ as a function of r, $\rho$, and $\epsilon_{t+1}$. 

## Answer

Using equation (2.18), we have:

$$
c_{t+1} = \frac{r}{1 + r - \rho} y_{t+1} - r d_t \quad \text{(1)}
$$

$$
c_t = \frac{r}{1 + r - \rho} y_t - r d_{t-1} \quad \text{(2)}
$$

Subtracting (2) from (1):

$$
c_{t+1} - c_t = \frac{r}{1 + r - \rho} (y_{t+1} - y_t) - r (d_t - d_{t-1}) \quad \text{(3)}
$$

Now plug in the AR(1) process for $y_t$:

$$
y_{t+1} = \rho y_t + \epsilon_{t+1}
$$

So:

$$
y_{t+1} - y_t = (\rho - 1) y_t + \epsilon_{t+1}
$$

Then:

$$
c_{t+1} - c_t = \frac{r}{1 + r - \rho} ((\rho - 1) y_t + \epsilon_{t+1}) - r(d_t - d_{t-1}) \quad \text{(4)}
$$

Now use the law of motion for external debt (equation 2.21):

$$
d_t - d_{t-1} = \frac{1 - \rho}{1 + r - \rho} y_t
$$

Substitute into the equation:

$$
c_{t+1} - c_t = \frac{r}{1 + r - \rho} ((\rho - 1) y_t + \epsilon_{t+1}) - r \cdot \frac{1 - \rho}{1 + r - \rho} y_t \quad \text{(5)}
$$

The terms involving \( y_t \) cancel:

$$
c_{t+1} - c_t = \frac{r}{1 + r - \rho} \epsilon_{t+1} \quad \text{(6)}
$$

::: {.callout-important title="Final Answer Summary"}
The innovation term is:

$$
\mu_{t+1} = c_{t+1} - c_t = \frac{r}{1 + r - \rho} \epsilon_{t+1}
$$
:::

