---
title: "Exercise 2.9"
subtitle: "Expected Output Changes and Permanent Income"
---
<a class="return-button" href="index.qmd">â¬… Return</a>

## Problem

Equation (2.27) expresses the difference between current and permanent income, $y_t - y^p_t$, as the present discounted value of expected future changes in the endowment. Present a step-by-step derivation of equation (2.27) starting from definitions (2.10) and (2.25). Comment on the cyclical properties of $y_t - y^p_t$ depending on whether the level or the change of $y_t$ follows an AR(1) process.

## Answer

Multiply equation (2.10) by $(1 + r)/r$.

$$
\frac{1 + r}{r} y^p_t = \sum_{j=0}^{\infty} \frac{\mathbb{E}_t y_{t+j}}{(1 + r)^j}
$$

Then split the sum,

$$
\frac{1 + r}{r} y^p_t = y_t + \sum_{j=1}^{\infty} \frac{\mathbb{E}_t y_{t+j}}{(1 + r)^j}
$$

Subtract $y^p_t$ from both sides

$$
\frac{1}{r} y^p_t = y_t - y^p_t + \sum_{j=1}^{\infty} \frac{\mathbb{E}_t y_{t+j}}{(1 + r)^j}
$$

Rearrange

$$
y_t - y^p_t = - \sum_{j=1}^{\infty} \frac{\mathbb{E}_t y_{t+j}}{(1 + r)^j} + \frac{1}{r} y^p_t
$$

Divide both sides of (2.10) by $r$ and then use the resulting expression to eliminate $\frac{1}{r} y^p_t$ from the above expression. This yields

$$
y_t - y^p_t = - \sum_{j=1}^{\infty} \frac{\mathbb{E}_t y_{t+j}}{(1 + r)^j} + \sum_{j=0}^{\infty} \frac{\mathbb{E}_t y_{t+j}}{(1 + r)^{j+1}} = - \sum_{j=1}^{\infty} \frac{1}{(1 + r)^j} \left[ \mathbb{E}_t y_{t+j} - \mathbb{E}_t y_{t+j-1} \right]
$$

Finally, use (2.25) to replace $\mathbb{E}_t y_{t+j} - \mathbb{E}_t y_{t+j-1}$ with $\mathbb{E}_t \Delta y_{t+j}$ to obtain equation (2.27).

If $y_t$ is AR(1), then as shown in section 2.2

$$
y^p_t = \frac{r}{1 + r - \rho} y_t
$$

so that

$$
y_t - y^p_t = \frac{1 - \rho}{1 + r - \rho} y_t
$$

Since $\rho \in (-1, 1)$, $\frac{1 - \rho}{1 + r - \rho} > 0$. It follows that $y_t - y^p_t$ is perfectly procyclical, $\text{corr}(y_t - y^p_t, y_t) = 1$. And $y_t - y^p_t$ inherits the serial correlation of $y_t$, $\text{corr}(y_t - y^p_t, y_{t-1} - y^p_{t-1}) = \text{corr}(y_t, y_{t-1}) = \rho$.

If $\Delta y_t$ is AR(1), then $\mathbb{E}_t \Delta y_{t+j} = \rho^j \Delta y_t$ for $j \geq 1$. By (2.27)

$$
y_t - y^p_t = - \frac{\rho}{1 + r - \rho} \Delta y_t
$$

Assuming (as in section 2.4) $\rho \in [0, 1)$, $-\frac{\rho}{1 + r - \rho} < 0$. It follows that $y_t - y^p_t$ is perfectly countercyclical, $\text{corr}(y_t - y^p_t, \Delta y_t) = -1$. Now $y_t - y^p_t$ inherits the serial correlation of $\Delta y_t$, $\text{corr}(y_t - y^p_t, y_{t-1} - y^p_{t-1}) = \text{corr}(\Delta y_t, \Delta y_{t-1}) = \rho$.